main/Semantics.v
@@ -18,7 +18,7 @@ Inductive step : ExecutionState -> ExecutionState -> Prop :=
     forall dest_addr amount value final_bm rest fenv env_stack c_st c_env new_bm src_addr old_bm,
       src_addr = (c_address c_st) ->
       old_bm = (balance_map fenv) ->
-      value = unfoldOptionZ (evalaexp (aexp_env fenv) amount) ->
+      value = unfold_option_z (eval_aexp (aexp_env fenv) amount) ->
       new_bm = (updateBalance old_bm dest_addr ((old_bm dest_addr) + value)) ->
       final_bm = (updateBalance new_bm src_addr ((new_bm src_addr) - value)) ->
       step (Transfer dest_addr amount :: rest, fenv, env_stack, c_st, c_env)
@@ -31,7 +31,7 @@ Inductive step : ExecutionState -> ExecutionState -> Prop :=
     forall called_addr msg_val value env env_stack c_st c_env c_st' fenv fcode fname rest,
       c_st' = c_env called_addr ->
       fcode = getFunctionCode ((fn_env c_st') fname) ->
-      value = unfoldOptionZ (evalaexp (aexp_env env) msg_val) ->
+      value = unfold_option_z (eval_aexp (aexp_env env) msg_val) ->
       fenv = mkEnv (Empty_Aexp_Env) (Empty_Bexp_Env) (rest) (balance_map env) (mkMsg value (c_address c_st)) ->
       step ((Function_Call called_addr fname msg_val) :: rest, env, env_stack, c_st, c_env) (fcode, fenv, (env, c_st) :: env_stack, c_st', c_env)
 
@@ -50,28 +50,39 @@ Inductive step : ExecutionState -> ExecutionState -> Prop :=
       env' = mkEnv aexp_env' (bexp_env env) (next_code env) (balance_map env) (msg_data env) ->
       step ((Declare_Aexp aexp_names) :: rest, env, env_stack, c_st, c_env) (rest, env', env_stack, c_st, c_env)
 
-| assign_aexp : 
-    forall a x v aexp_env' rest env env' env_stack c_st c_env,
-      v = unfoldOptionZ (evalaexp (aexp_env env) a) ->
-      aexp_env' = updateAexp (aexp_env env) x v ->
+| assign_aexp_local : (* variable is local to function env *)
+    forall a x v aexp_env' rest env env' env_stack c_st c_env string_id,
+      string_id = unfold_aexp_id x ->
+      v = unfold_option_z (eval_aexp (aexp_env env) a) ->
+      aexp_env' = update_aexp (aexp_env env) string_id v ->
       env' = mkEnv aexp_env' (bexp_env env) (next_code env) (balance_map env) (msg_data env) ->
       step (Assignment_Aexp x a :: rest, env, env_stack, c_st, c_env) (rest, env', env_stack, c_st, c_env)
 
+| assign_aexp_contract : (* variable is contract member *)
+    forall a x v contract_aexp_env local_aexp_env rest env env' env_stack c_st c_st' c_env string_id,
+      string_id = unfold_aexp_id x ->
+      v = unfold_option_z (eval_aexp (aexp_env env) a) ->
+      local_aexp_env = update_aexp (aexp_env env) string_id v ->
+      contract_aexp_env = update_aexp (aexp_vars c_st) string_id v ->
+      env' = mkEnv local_aexp_env (bexp_env env) (next_code env) (balance_map env) (msg_data env) ->
+      c_st' = replace_contract_aexp_env c_st contract_aexp_env ->
+      step (Assignment_Aexp x a :: rest, env, env_stack, c_st, c_env) (rest, env', env_stack, c_st', c_env)
+
 | assign_bexp :
     forall b x v bexp_env' rest env env' env_stack c_st c_env,
-      v = unfoldOptionBool (evalbexp (aexp_env env) (bexp_env env) b) ->
-      bexp_env' = updateBexp (bexp_env env) x v ->
+      v = unfold_option_bool (eval_bexp (aexp_env env) (bexp_env env) b) ->
+      bexp_env' = update_bexp (bexp_env env) x v ->
       env' = mkEnv (aexp_env env) (bexp_env') (next_code env) (balance_map env) (msg_data env) ->
       step (Assignment_Bexp x b :: rest, env, env_stack, c_st, c_env) (rest, env', env_stack, c_st, c_env)
 
 | if_true :
     forall b s1 s2 rest env env_stack c_st c_env,
-      Some true = (evalbexp (aexp_env env) (bexp_env env) b) ->
+      Some true = (eval_bexp (aexp_env env) (bexp_env env) b) ->
       step (IfThenElse b s1 s2 :: rest, env, env_stack, c_st, c_env) (s1 ++ rest, env, env_stack, c_st, c_env)
 
 | if_false :
     forall b s1 s2 rest env env_stack c_st c_env,
-      Some false = (evalbexp (aexp_env env) (bexp_env env) b) ->
+      Some false = (eval_bexp (aexp_env env) (bexp_env env) b) ->
       step (IfThenElse b s1 s2 :: rest, env, env_stack, c_st, c_env) (s2 ++ rest, env, env_stack, c_st, c_env)
 
 | while:
@@ -91,6 +102,7 @@ Inductive steps : ExecutionState -> ExecutionState -> Prop :=
 
 
 (** address.transfer(amount) *)
+Section transfer.
 
 Let receiver := "addr".
 Let amount := Int 1.
@@ -114,11 +126,15 @@ Proof.
   }
   Qed.
 
+End transfer.
+
+Import ListNotations.
 
 
+(** function call *)
+Section function_call.
 
-(** Setup *)
-Let called_fn_code := Declare_Aexp ("fn_a" :: nil)  :: nil.
+Let called_fn_code := [Declare_Aexp [("fn_a", None)]].
 Let called_fn := "called_fn".
 Let called_contract_funs_env := defineFunction Empty_Functions_Env called_fn (Body called_fn_code).
 Let called_contract_address := "called_contract".
@@ -126,20 +142,19 @@ Let called_contract_state := mkContractState called_contract_address called_cont
 
 Let calling_contract_state := Default_ContractState.
 
-Let example2_contracts_env := updateContractsEnv Empty_ContractsEnv called_contract_address called_contract_state.
+Let example_contracts_env := updateContractsEnv Empty_ContractsEnv called_contract_address called_contract_state.
 
 Let msg_val := Int 0.
 Let msg_val_z := 0%Z.
-Let current_vars := "a" :: nil.
+Let current_vars : list (string * option Z) := [("a", None)].
 Let current_code := (Declare_Aexp current_vars) :: (Function_Call called_contract_address called_fn msg_val) :: nil.
 
 Let fn_env_before_call := (replace_aexp_env Empty_FunctionEnv (declareAexpList (aexp_env Empty_FunctionEnv) current_vars)).
 Let called_fn_env := replace_msg_data Empty_FunctionEnv (mkMsg  msg_val_z (c_address calling_contract_state)).
 
-(** function call *)
 Example Step_Into_Call :
-  steps (current_code, Empty_FunctionEnv, nil, calling_contract_state, example2_contracts_env)
-        (called_fn_code, called_fn_env, (fn_env_before_call, calling_contract_state) :: nil, called_contract_state, example2_contracts_env).
+  steps (current_code, Empty_FunctionEnv, nil, calling_contract_state, example_contracts_env)
+        (called_fn_code, called_fn_env, (fn_env_before_call, calling_contract_state) :: nil, called_contract_state, example_contracts_env).
 Proof.
   eapply trans.
   - eapply declare_aexp; eauto.
@@ -148,26 +163,27 @@ Proof.
     * apply refl.
 Qed.
 
-
+End function_call.
 
 
 (** function exit *)
+Section function_exit.
 
 Let fenv_with_remaining_code := replace_next_code Empty_FunctionEnv (Skip :: nil).
-Let called_contract_address2 := "called_contract".
-Let called_contract_state2 := mkContractState called_contract_address2 Empty_Functions_Env Empty_Aexp_Env Empty_Bexp_Env.
+Let called_contract_address := "called_contract".
+Let called_contract_state := mkContractState called_contract_address Empty_Functions_Env Empty_Aexp_Env Empty_Bexp_Env.
 
-Let calling_contract_state2 := Default_ContractState.
+Let calling_contract_state := Default_ContractState.
 
-Let example_contracts_env3 := updateContractsEnv 
-(updateContractsEnv Empty_ContractsEnv called_contract_address2 called_contract_state2)
-Default_Address calling_contract_state2.
+Let example_contracts_env := updateContractsEnv 
+(updateContractsEnv Empty_ContractsEnv called_contract_address called_contract_state)
+Default_Address calling_contract_state.
 
 Example Function_exit:
-  steps (nil, Empty_FunctionEnv, (fenv_with_remaining_code, calling_contract_state2)::nil,
-  called_contract_state2, example_contracts_env3)
+  steps (nil, Empty_FunctionEnv, (fenv_with_remaining_code, calling_contract_state)::nil,
+  called_contract_state, example_contracts_env)
   (next_code fenv_with_remaining_code, fenv_with_remaining_code, nil,
-   calling_contract_state2, example_contracts_env3).
+   calling_contract_state, example_contracts_env).
 Proof.
   eapply trans.
   {
@@ -178,11 +194,63 @@ Proof.
   }
   Qed.
 
+End function_exit.
+
+
+(** Contract and local variable *)
+Section contract_and_local_var.
+
+Let called_fn_code := [Declare_Aexp [("local_a", Some 100%Z)]; Assignment_Aexp (AId "contract_a") (AId "local_a")].
+Let called_fn := "called_fn".
+Let called_contract_funs_env := defineFunction Empty_Functions_Env called_fn (Body called_fn_code).
+Let called_contract_address := "called_contract".
+Let contract_aexp_env := declareAexpList Empty_Aexp_Env [("contract_a", None)].
+Let called_contract_state := 
+mkContractState called_contract_address called_contract_funs_env contract_aexp_env Empty_Bexp_Env.
+Let final_contract_state :=
+replace_contract_aexp_env called_contract_state (update_aexp contract_aexp_env (Some "contract_a") 100%Z).
+Let initial_fn_env := replace_aexp_env Empty_FunctionEnv contract_aexp_env.
+Let final_fn_env := 
+replace_aexp_env initial_fn_env (update_aexp (update_aexp contract_aexp_env (Some "local_a") 100%Z) (Some "contract_a") 100%Z).
+
+Example contract_and_local_var:
+steps (called_fn_code, initial_fn_env, [], called_contract_state, Empty_ContractsEnv)
+      ([], final_fn_env, [], final_contract_state, Empty_ContractsEnv).
+Proof.
+  eapply trans.
+  {
+    eapply declare_aexp; eauto.
+  }
+  eapply trans.
+  eapply assign_aexp_contract; eauto.
+  eapply refl.
+Qed.
+
+End contract_and_local_var.
+
 
 (** Code sample *)
+Section tricky_transfer.
+
+Let address_Alice := "0xA".
+Let balance_map_Alice := updateBalance Empty_BalanceMap address_Alice 10%Z. 
+
+Let address_Jane := "0xF".
+Let balance_map_Jane := updateBalance Empty_BalanceMap address_Jane 20%Z. 
+
+Let fun_code_Alice := [Transfer address_Jane (Int 10%Z)].
+Let fun_name_Alice := "Alice_Fun".
+Let funs_env_Alice_contract := defineFunction Empty_Functions_Env fun_name_Alice (Body fun_code_Alice).
+
+
+Example Tricky_Transfer:
+steps ()
+().
+Proof.
+
+End tricky_transfer.
 
 (*
-
 (Declare_Aexp "a" :: "b")::
 (Assignment_Aexp "a" (Int 1))::
 
@@ -191,7 +259,6 @@ IfThenElse (Aexp_Gt (AId "a") (AId "b"))
 (Function_Call "addr" "send" (AId "b"))::nil  (* else *)
 
 ::nil 
-
 *)
 
 
